pure/Learn.Option.fst
@@ -1,5 +1,10 @@
 module Learn.Option
 
+let map #a #b (f : a -> b) (x : option a) : option b
+  = match x with
+  | None   -> None
+  | Some x -> Some (f x)
+
 let bind #a #b (x : option a) (f : a -> option b) : option b
   = match x with
   | None   -> None
